# baseURI: http://promsns.org/def/proms
# imports: http://purl.org/dc/elements/1.1/
# imports: http://purl.org/dc/terms/
# imports: http://purl.org/vocab/vann/
# imports: http://purl.org/vocommons/voaf#
# imports: http://rdfs.org/ns/void
# imports: http://www.w3.org/2000/01/rdf-schema
# imports: http://www.w3.org/ns/prov
# imports: http://xmlns.com/foaf/0.1/

@prefix :        <http://promsns.org/def/proms#> .
@prefix cc:      <http://creativecommons.org/ns#> .
@prefix dc:      <http://purl.org/dc/elements/1.1/> .
@prefix dct:     <http://purl.org/dc/terms/> .
@prefix foaf:    <http://xmlns.com/foaf/0.1/> .
@prefix ns:      <http://www.w3.org/2006/vcard/ns#> .
@prefix owl:     <http://www.w3.org/2002/07/owl#> .
@prefix prov:    <http://www.w3.org/ns/prov#> .
@prefix rdf:     <http://www.w3.org/1999/02/22-rdf-syntax-ns#> .
@prefix rdfs:    <http://www.w3.org/2000/01/rdf-schema#> .
@prefix skos:    <http://www.w3.org/2004/02/skos/core#> .
@prefix vann:    <http://purl.org/vocab/vann/> .
@prefix voaf:    <http://purl.org/vocommons/voaf#> .
@prefix void:    <http://rdfs.org/ns/void#> .
@prefix xsd:     <http://www.w3.org/2001/XMLSchema#> .

<http://promsns.org/def/proms>
      rdf:type owl:Ontology , voaf:Vocabulary ;
      rdfs:comment "This ontology is an extension to the PROV ontology. It adds several classes that constrain the outputs from systems that generate provenance data and allow outputs from heterogeneous systems to be stored in a single provenance store."@en ;
      rdfs:label "Provenance Management System Ontology"@en ;
      dc:creator "Nicholas J. Car"^^xsd:string ;
      dc:description "All classes in this ontology are subclasses (specialisations) of PROV classes."@en ;
      dc:publisher "CSIRO"^^xsd:string ;
      dc:rights "Copyright 2014 CSIRO"^^xsd:string ;
      dc:title "Provenance Management System Ontology"^^xsd:string ;
      dct:created "2014"^^xsd:gYear ;
      dct:hasPart "EntityComponent"^^xsd:string , "reportingSystem"^^xsd:string , "ServiceEntity"^^xsd:string , "owner"^^xsd:string , "InternalReport"^^xsd:string , "nativeId"^^xsd:string , "Report"^^xsd:string , "componentOf"^^xsd:string , "query"^^xsd:string , "startingActivity"^^xsd:string , "ReportingSystem"^^xsd:string , "BasicReport"^^xsd:string , "endingActivity"^^xsd:string , "ExternalReport"^^xsd:string ;
      dct:license <https://wiki.csiro.au/pages/viewpage.action?pageId=663847169> ;
      dct:modified "2015-06-29"^^xsd:string ;
      vann:preferredNamespacePrefix
              "proms"^^xsd:string ;
      vann:preferredNamespaceUri
              "http://promsns.org/def/proms#"^^xsd:string ;
      voaf:extends prov: ;
      void:uriSpace "http://promsns.org/def/proms#"^^rdf:XMLLiteral ;
      void:vocabulary "http://promsns.org/def/proms"^^xsd:string ;
      owl:imports vann: , <http://www.w3.org/ns/prov> , voaf: , dct: , <http://rdfs.org/ns/void> , foaf: , <http://www.w3.org/2000/01/rdf-schema> , dc: ;
      owl:versionInfo "1.0"^^xsd:string .

:BasicReport
      rdf:type owl:Class ;
      rdfs:comment "A Report for which no other information is known that its ReportingSystem's nativeId and a generatedAtTime. It is little more than a log entry with few details."@en ;
      rdfs:isDefinedBy <http://promsns.org/def/proms> ;
      rdfs:label "Basic Report"@en ;
      rdfs:subClassOf :Report ;
      rdfs:subClassOf
              [ rdf:type owl:Restriction ;
                owl:allValuesFrom xsd:string ;
                owl:onProperty rdfs:comment
              ] .

:EntityComponent
      rdf:type owl:Class ;
      rdfs:comment "EntityComponents are sub-members of PROV Entities not derived from them such as files within an Entity that is a file bundle or elements within a database that is an Entity."@en ;
      rdfs:isDefinedBy <http://promsns.org/def/proms> ;
      rdfs:label "Entity Component" ;
      rdfs:subClassOf prov:Entity ;
      rdfs:subClassOf
              [ rdf:type owl:Restriction ;
                owl:allValuesFrom prov:Entity ;
                owl:onProperty :componentOf
              ] .

:ExternalReport
      rdf:type owl:Class ;
      rdfs:comment "A Report for which the identities of the data items (Entities) that the ReportingSystem that generated it are known but no internal process steps. An ExternalReport is a 'back box' with regards to its ReportingSystem's internal processes."^^xsd:string ;
      rdfs:isDefinedBy <http://promsns.org/def/proms> ;
      rdfs:label "External Report"@en ;
      rdfs:subClassOf :Report ;
      rdfs:subClassOf
              [ rdf:type owl:Restriction ;
                owl:allValuesFrom prov:Activity ;
                owl:onProperty :startingActivity
              ] ;
      rdfs:subClassOf
              [ rdf:type owl:Restriction ;
                owl:allValuesFrom prov:Activity ;
                owl:onProperty :endingActivity
              ] .

:InternalReport
      rdf:type owl:Class ;
      rdfs:comment "A Report for which details of the ReportingSystem that generated its internal details are known. The internal details are a series of one or more prov:Activity class instances with appropriate handover prov:Entity class instances with at least known input Entities to the first Activity and Entity outputs from the last Activity."@en ;
      rdfs:isDefinedBy <http://promsns.org/def/proms> ;
      rdfs:label "Internal Report"@en ;
      rdfs:subClassOf :Report ;
      rdfs:subClassOf
              [ rdf:type owl:Restriction ;
                owl:allValuesFrom prov:Activity ;
                owl:onProperty :endingActivity
              ] ;
      rdfs:subClassOf
              [ rdf:type owl:Restriction ;
                owl:allValuesFrom prov:Activity ;
                owl:onProperty :startingActivity
              ] .

:Report
      rdf:type owl:Class ;
      rdfs:comment "Reports are the outputs of a single ReportingSystem operation. They are a single graph describing some provenance for the output od the ReportingSystem's operation's outputs."@en ;
      rdfs:isDefinedBy <http://promsns.org/def/proms> ;
      rdfs:label "Report"@en ;
      rdfs:subClassOf prov:Entity ;
      rdfs:subClassOf
              [ rdf:type owl:Restriction ;
                owl:allValuesFrom :ReportingSystem ;
                owl:onProperty :reportingSystem
              ] ;
      rdfs:subClassOf
              [ rdf:type owl:Restriction ;
                owl:allValuesFrom xsd:string ;
                owl:onProperty :nativeId
              ] ;
      rdfs:subClassOf
              [ rdf:type owl:Restriction ;
                owl:allValuesFrom xsd:string ;
                owl:onProperty dc:title
              ] .

:ReportingSystem
      rdf:type owl:Class ;
      rdfs:comment "A ReportingSystem is a SoftwareAgent, computer or other system that is able to produce Reports, therefore it is a system that is able to trace some level of provenance for processes that it undertakes. It must be acting on behalf of a person: reportingSsytemOwner."@en ;
      rdfs:isDefinedBy <http://promsns.org/def/proms> ;
      rdfs:label "Reporting System"@en ;
      rdfs:subClassOf prov:Agent ;
      rdfs:subClassOf
              [ rdf:type owl:Restriction ;
                owl:allValuesFrom xsd:string ;
                owl:onProperty dc:title
              ]  .

:ServiceEntity
      rdf:type owl:Class ;
      rdfs:comment "ServiceEntities are entities delivered by a service thus it is expected that the data that this Entity subclass representes is available via a query."@en ;
      rdfs:isDefinedBy <http://promsns.org/def/proms> ;
      rdfs:label "Service delivered Entity"^^xsd:string ;
      rdfs:subClassOf prov:Entity ;
      rdfs:subClassOf
              [ rdf:type owl:Restriction ;
                owl:allValuesFrom xsd:dateTime ;
                owl:onProperty :queriedAtTime
              ] ;
      rdfs:subClassOf
              [ rdf:type owl:Restriction ;
                owl:allValuesFrom rdfs:Resource ;
                owl:onProperty :serviceBaseUri
              ] ;
      rdfs:subClassOf
              [ rdf:type owl:Restriction ;
                owl:allValuesFrom xsd:string ;
                owl:onProperty :query
              ] .

:componentOf
      rdf:type owl:ObjectProperty ;
      rdfs:comment "An EntityComponent must be linked to its parent Entity"^^xsd:string ;
      rdfs:domain :EntityComponent ;
      rdfs:isDefinedBy <http://promsns.org/def/proms> ;
      rdfs:label "component of"^^xsd:string ;
      rdfs:range prov:Entity ;
      skos:prefLabel "component of"^^xsd:string .

:endingActivity
      rdf:type owl:ObjectProperty ;
      rdfs:comment "The final Activity, based on endedAtTime, described by the Report."^^xsd:string ;
      rdfs:domain :Report ;
      rdfs:isDefinedBy <http://promsns.org/def/proms> ;
      rdfs:label "ending Activity"^^xsd:string ;
      rdfs:range prov:Activity ;
      skos:prefLabel "ending Activity"^^xsd:string .
	  
:generatedAtTime
	  rdf:type owl:ObjectProperty ;
      rdfs:comment "The time at which the report was generated."^^xsd:string ;
      rdfs:domain :Report ;
      rdfs:isDefinedBy http://www.w3.org/ns/prov#generatedAtTime> ;
      rdfs:label "generated At Time"^^xsd:string ;
      rdfs:range <http://www.w3.org/2001/XMLSchema#dateTime> ;
      skos:prefLabel "generated At Time"^^xsd:string .

:nativeId
      rdf:type owl:ObjectProperty ;
      rdfs:comment "The ID the ReportingSystem allocates to the job that generated this Report"^^xsd:string ;
      rdfs:domain :Report ;
      rdfs:isDefinedBy <http://promsns.org/def/proms> ;
      rdfs:label "native ID"^^xsd:string ;
      rdfs:range xsd:string ;
      skos:prefLabel "native ID"^^xsd:string .

:owner
      rdf:type owl:ObjectProperty ;
      rdfs:comment "The person (individual) who owns, or is responsible for, a particular ReportingSystem"^^xsd:string ;
      rdfs:domain :ReportingSystem ;
      rdfs:isDefinedBy <http://promsns.org/def/proms> ;
      rdfs:label "owner"^^xsd:string ;
      rdfs:range foaf:Person ;
      skos:prefLabel "owner"^^xsd:string .

:queriedAtTime
      rdf:type owl:ObjectProperty ;
      rdfs:comment "This is the time at which the EntityService's service was actually queried. This may be quite a different time from the Entity's createdAtTime or any created time of the EntityService's service. It is similar to the \"Accessed At\" property of academic paper's web page citations."^^xsd:string ;
      rdfs:domain :ServiceEntity ;
      rdfs:isDefinedBy <http://promsns.org/def/proms> ;
      rdfs:label "queried at time"^^xsd:string ;
      rdfs:range xsd:dateTime ;
      skos:prefLabel "queried at time"^^xsd:string .

:query
      rdf:type owl:ObjectProperty ;
      rdfs:comment "The query used to generate the data represented by a ServiceEntity"^^xsd:string ;
      rdfs:domain :ServiceEntity ;
      rdfs:isDefinedBy <http://promsns.org/def/proms> ;
      rdfs:label "query"^^xsd:string ;
      rdfs:range xsd:string ;
      skos:prefLabel "query"^^xsd:string .

:reportingSystem
      rdf:type owl:ObjectProperty ;
      rdfs:comment "Each Report must be associated with a ReportingSystem instance"^^xsd:string ;
      rdfs:domain :Report ;
      rdfs:isDefinedBy <http://promsns.org/def/proms> ;
      rdfs:label "from reporting system"@en ;
      rdfs:range :ReportingSystem .

:serviceBaseUri
      rdf:type owl:ObjectProperty ;
      rdfs:domain :ServiceEntity ;
      rdfs:isDefinedBy <http://promsns.org/def/proms> ;
      rdfs:label "service base uri"^^xsd:string ;
      rdfs:range xsd:anyURI ;
      skos:prefLabel "service base uri"^^xsd:string .

:startingActivity
      rdf:type owl:ObjectProperty ;
      rdfs:comment "The initial Activity, based on startedAtTime, described by the Report."^^xsd:string ;
      rdfs:domain :Report ;
      rdfs:isDefinedBy <http://promsns.org/def/proms> ;
      rdfs:label "starting Activity"^^xsd:string ;
      rdfs:range prov:Activity ;
      skos:prefLabel "starting Activity"^^xsd:string .
	  
:validation
      rdf:type owl:ObjectProperty ;
      rdfs:comment "Each ReportingSystem must list the file (=== class) name of its validation code"^^xsd:string ;
      rdfs:domain :ReportingSystem ;
      rdfs:isDefinedBy <http://promsns.org/def/proms> ;
      rdfs:label "validated according to"@en ;
      rdfs:range xsd:string .